FormaleSystemeInLean/Finset.lean
@@ -1,0 +1,172 @@
+import FormaleSystemeInLean.Set
+import FormaleSystemeInLean.List
+
+def Finset' (α : Type u) := List α
+
+instance : Membership α (Finset' α) where
+  mem s a := s.Mem a
+
+def Finset.eq (l k : Finset' α) : Prop :=
+  ∀ (a : α), a ∈ l ↔ a ∈ k
+
+def Finset.eq.eqv : Equivalence (@Finset.eq α) where
+  refl := by
+    unfold eq; intro X a; rfl
+  symm := by
+    unfold eq; intro X Y h x; symm; exact h x
+  trans := by
+    unfold eq
+    intro X Y Z eq_XY eq_YZ x; rw [eq_XY]; exact eq_YZ x
+
+instance Finset.instSetoid (α : Type u) : Setoid (Finset' α) where
+  r := Finset.eq
+  iseqv := Finset.eq.eqv
+
+def Finset (α : Type u) : Type u := Quotient (@Finset.instSetoid α)
+
+def Finset.mk (l : Finset' α) : Finset α := Quotient.mk _ l
+
+theorem Finset.perm_iff_eq [DecidableEq α] (l k : Finset' α) (eq : Finset.eq l k) : l.removeDups.Perm k.removeDups := by
+  unfold Finset.eq at eq
+  have mem_rd_l := List.mem_removeDups l
+  have mem_rd_k := List.mem_removeDups k
+  have count_l := List.removeDups_count l
+  have count_k := List.removeDups_count k
+  have count_eq : ∀ a, l.removeDups.count a = k.removeDups.count a := by
+    intro a
+    by_cases a_mem : a ∈ l
+    . specialize count_l a a_mem
+      have a_mem_k := (eq a).mp a_mem
+      specialize count_k a a_mem_k
+      rw [count_l, count_k]
+    . have a_nmem : ¬a ∈ l.removeDups := by
+        intro contra
+        specialize mem_rd_l a
+        have aux := mem_rd_l.mpr contra
+        contradiction
+      have a_nmem2 : ¬a ∈ k.removeDups := by
+        intro contra
+        specialize mem_rd_k a
+        have aux := (eq a).mpr (mem_rd_k.mpr contra)
+        contradiction
+      have count_l : l.removeDups.count a = 0 := by
+        rw [List.count_eq_zero]; exact a_nmem
+      have count_k : k.removeDups.count a = 0 := by
+        rw [List.count_eq_zero]; exact a_nmem2
+      rw [count_k, count_l]
+  simp only [List.perm_iff_count]
+  exact count_eq
+
+theorem Finset.length_eq_if_eq [DecidableEq α] (l k : Finset' α) (eq : Finset.eq l k) : l.removeDups.length = k.removeDups.length := by
+  have perm := perm_iff_eq l k eq
+  apply List.Perm.length_eq
+  exact perm
+
+def Finset.card [DecidableEq α] : Finset α -> Nat :=
+  Quot.lift
+    (fun l' => l'.removeDups.length)
+    (by
+      intro l k h
+      unfold Setoid.r instSetoid eq at h
+      simp only at h
+      have eq : Finset.eq l k := by unfold eq; exact h
+      have aux := length_eq_if_eq l k eq
+      grind
+    )
+
+def Finset.mem (a : α) : Finset α -> Prop :=
+  Quot.lift
+    (fun s => a ∈ s)
+    (by
+      intro x y h
+      unfold Setoid.r instSetoid eq at h
+      simp only at h
+      grind
+    )
+
+def Finset.union : Finset α -> Finset α -> Finset α :=
+  Quotient.lift₂
+    (fun a b => Finset.mk (a.append b))
+    (by
+      intro u v w x eq_vx eq_uw
+      simp only [List.append_eq]
+      unfold mk Quotient.mk Setoid.r instSetoid Finset.eq
+      simp
+      simp only [HasEquiv.Equiv, Setoid.r, eq] at *
+      have aux : ∀ a, a ∈ (u.append v) ↔ a ∈ (w.append x) := by
+        intro a
+        simp only [List.append_eq, List.mem_append]
+        grind
+      have test : Finset.eq (u.append v) (w.append x) := by
+        unfold eq; exact aux
+      have aux2 := Quot.sound test
+      exact aux2
+    )
+
+def Finset.ext : Finset α -> Finset α -> Prop :=
+  Quotient.lift₂
+    (fun a b => Finset.eq a b)
+    (by
+      intro a1 a2 b1 b2 eq1 eq2
+      simp only [HasEquiv.Equiv, Setoid.r, eq] at *
+      simp only [eq_iff_iff]
+      grind)
+
+
+
+def Finset.insert (a : α) : Finset α → Finset α :=
+  Quot.lift
+    (fun s => Finset.mk (a::s))
+    (by
+      intro x y h
+      unfold Setoid.r instSetoid eq at h
+      simp only at *
+      unfold mk Quotient.mk Setoid.r instSetoid eq
+      simp
+      have aux : Finset.eq (a::x) (a::y) := by
+        unfold eq
+        intro c
+        specialize h c
+        rw [List.mem_cons]
+        by_cases hc : c = a
+        . rw [hc]
+          simp only [true_or, true_iff]
+          rw [List.mem_cons]
+          apply Or.inl; rfl
+        . simp only [hc, false_or, h]
+          rw [List.mem_cons]
+          simp only [iff_or_self]
+          grind
+      have aux2 := Quot.sound aux
+      exact aux2)
+
+
+
+instance : EmptyCollection (Finset α) where
+  emptyCollection := Finset.mk []
+
+instance : Membership α (Finset α) where
+  mem s a := s.mem a
+
+instance : Union (Finset α) where
+  union X Y := Finset.union X Y
+
+instance : HasSubset (Finset α) where
+  Subset A B := ∀ e, e ∈ A -> e ∈ B
+
+theorem test (X Y : Finset α) : X = Y -> (∀ a, a ∈ X ↔ a ∈ Y) := by
+  intro a; grind
+
+theorem eq_iff (X Y : Finset α)  : X = Y ↔ Finset.ext X Y := by
+  constructor
+  . intro eq
+    have aux := test X Y eq
+    unfold Finset.ext
+    simp only [Quotient.lift₂, Quotient.lift, Finset.eq]
+
+    sorry
+  .
+    sorry
+
+instance [DecidableEq α] (x : α) (S : Finset α) : Decidable (x ∈ S) :=
+  Quot.recOnSubsingleton S (fun l => List.instDecidableMemOfLawfulBEq x l)
